\begin{frame}
\frametitle{foldl}

The \lstinline[basicstyle=\ttfamily]$foldl$ function is a machine that requires three values:
\begin{enumerate}
\item \lstinline[basicstyle=\ttfamily]$f :: b -> a -> b$
\item \lstinline[basicstyle=\ttfamily]$z :: b$
\item \lstinline[basicstyle=\ttfamily]$list :: List a$
\end{enumerate}

It will give you back a value of the type \lstinline[basicstyle=\ttfamily]$b$.

\hrulefill

\lstinline[basicstyle=\ttfamily]$foldl :: (b -> a -> b) -> b -> List a -> b$

\end{frame}


\begin{frame}
\frametitle{foldl}

\begin{block}{What does this machine do?}

\begin{itemize}
\item OK, so \lstinline[basicstyle=\ttfamily]$foldl$ takes three arguments.
\item But what does this machine do to those three arguments to compute the return value?
\end{itemize}


\end{block}

\end{frame}


\begin{frame}
\frametitle{foldl}

\begin{block}{A standard loop, exactly in a way in which we are familiar}
\lstinputlisting[label=lst:foldl-loop,basicstyle=\ttfamily]{source/foldl-loop}
\end{block}

\end{frame}


\begin{frame}
\frametitle{foldl}
\framesubtitle{example \textemdash product}

\begin{block}{Really, is that all?}
To compute the product of the list, let:
\begin{enumerate}
\item \lstinline[basicstyle=\ttfamily]$f = *$
\item \lstinline[basicstyle=\ttfamily]$z = 1$
\end{enumerate}
\end{block}

\end{frame}


\begin{frame}[fragile]
\frametitle{foldl}
\framesubtitle{example \textemdash product}

\begin{block}{Yes, that is all}
\lstinputlisting[label=lst:foldl-loop-product,basicstyle=\ttfamily]{source/foldl-loop-product}
\end{block}

\hrulefill

\begin{lstlisting}
product list =
  foldl (*) 1 list
\end{lstlisting}

\end{frame}


\begin{frame}
\frametitle{foldl}
\framesubtitle{example \textemdash reverse}

\begin{block}{Another examples}
To reverse a list, let:
\begin{enumerate}
\item \lstinline[basicstyle=\ttfamily]$f = \\xs x -> x : xs$
\item \lstinline[basicstyle=\ttfamily]$z = Nil$
\end{enumerate}
\end{block}

\end{frame}


\begin{frame}[fragile]
\frametitle{foldl}
\framesubtitle{example \textemdash reverse}

\begin{block}{Reversing a cons list}
\lstinputlisting[label=lst:foldl-loop-reverse,basicstyle=\ttfamily]{source/foldl-loop-reverse}
\end{block}

\hrulefill

\begin{lstlisting}
reverse list =
  foldl (\xs x -> x : xs) [] list
\end{lstlisting}

\end{frame}


\begin{frame}[fragile]
\frametitle{foldl}
\framesubtitle{observations}

\begin{block}{Observations about \lstinline[basicstyle=\ttfamily]$foldl$}
\begin{itemize}
\item We might compute the \lstinline[basicstyle=\ttfamily]$length$ of a list with \lstinline[basicstyle=\ttfamily]$foldl$.
\item We might compute the \lstinline[basicstyle=\ttfamily]$sum$ of a list with \lstinline[basicstyle=\ttfamily]$foldl$.
\item Importantly, \lstinline[basicstyle=\ttfamily]$foldl$ \textbf{will never work on an infinite list}.
\end{itemize}
\end{block}

\hrulefill

There is nothing more or less to \lstinline[basicstyle=\ttfamily]$foldl$ than what has just been described.

\end{frame}
